

Standard Diffusion

$$\frac{\partial c}{\partial t} = D \nabla_c^2 - kc$$

Concentration gradient

Proportional metabolism

Since it is 1D,

$$\frac{\partial c}{\partial t} = D \frac{\partial^2 c}{\partial x^2} - kc \quad \text{--- (1)}$$

Since the boundary condition at $x=0$ is $c_0 \neq 0$, it's non-homogenous, so, splitting up the solution into

→ Transient solution $c_T(x, t)$

→ Steady state $c_\infty(x)$

$$\text{So, } c(x, t) = c_T(x, t) + c_\infty(x) \quad \text{--- (2)}$$

Solving for steady state, we set $\frac{\partial c}{\partial t} = 0$

$$\rightarrow 0 = D \frac{d^2 c_\infty}{dx^2} - k c_\infty$$

$$\rightarrow \frac{d^2 c_\infty}{dx^2} - \frac{k}{D} c_\infty = 0$$

Using general form $[f'' - k^2 f = 0 \rightarrow f(x) = A \cosh(kx) + B \sinh(kx)]$

$$\rightarrow c_\infty(x) = A \cosh\left(\sqrt{\frac{k}{D}} x\right) + B \sinh\left(\sqrt{\frac{k}{D}} x\right)$$

→ (S1)

Applying boundary conditions

$$c_{\infty}(0) = c_0 \rightarrow A(1) + B(0) = c_0 \rightarrow A = c_0$$

$$c_{\infty}(L) = 0 \rightarrow c_0 \cosh\left(\sqrt{\frac{k}{D}} L\right) + B \sinh\left(\sqrt{\frac{k}{D}} L\right) = 0$$

$$\hookrightarrow B = -c_0 \frac{\cosh\left(\sqrt{\frac{k}{D}} L\right)}{\sinh\left(\sqrt{\frac{k}{D}} L\right)} = -c_0 \coth\left(\sqrt{\frac{k}{D}} L\right)$$

Plugging A and B to (S1),

$$c_{\infty}(x) = c_0 \cosh\left(\sqrt{\frac{k}{D}} x\right) - c_0 \coth\left(\sqrt{\frac{k}{D}} L\right) \sinh\left(\sqrt{\frac{k}{D}} x\right)$$

Using $[\sinh(A - B) = \sinh A \cosh B - \cosh A \sinh B]$,

$$c_{\infty}(x) = c_0 \frac{\sinh\left(\sqrt{\frac{k}{D}} (L - x)\right)}{\sinh\left(\sqrt{\frac{k}{D}} L\right)} \quad \text{--- (S2)}$$

Now for the transient solution,

Let's place $C = C_T + c_{\infty}$ into (1)

$$\frac{\partial (C_T + c_{\infty})}{\partial t} = D \frac{\partial^2 (C_T + c_{\infty})}{\partial x^2} - k(C_T + c_{\infty})$$

Since c_{∞} is not a function of t ,

$$\rightarrow \frac{\partial C_T}{\partial t} = D \frac{\partial^2 C_T}{\partial x^2} - k C_T \quad \text{--- (T1)}$$

For new boundary conditions,

$$c_T(0,t) = c(0,t) - c_\infty(0) = c_0 - c_0 = 0$$

$$c_T(L,t) = c(L,t) - c_\infty(L) = 0 - 0 = 0$$

$$c_T(x,0) = c(x,0) - c_\infty(x) = 0 - c_\infty(x) = -c_\infty(x)$$

These are homogeneous, so we can separate the variables like

$$C_T(x,t) = X(x) T(t) \quad \text{--- } \textcircled{T2}$$

In $\textcircled{T1}$,

$$X T' = D X'' T - k X T$$

$$\rightarrow \frac{T'}{T} = D \frac{X''}{X} - k$$

$$\rightarrow \frac{T'}{T} + k = D \frac{X''}{X} = -\lambda D$$

Separation constant to ensure decaying solutions

So we have

$$\text{Spatial: } X'' = -\lambda X$$

$$\text{Time: } \frac{T'}{T} + k = -\lambda D$$

For spatial, using conditions $x(0)=0$, $x(L)=0$, it leads to standard sine eigenfunctions

$$X_n(x) = \sin\left(\frac{n\pi x}{L}\right), \quad \lambda_n = \left(\frac{n\pi}{L}\right)^2, \quad n=1,2,3,\dots$$

Time then becomes

$$\frac{T'}{T} + k = -D \lambda_n$$

$$\rightarrow T' + (k + D\lambda_n) T = 0$$

Using the standard form ...

$$T_n(t) = e^{-t(D(\frac{n\pi}{L})^2 + k)}$$

Thus, (T2) becomes,

$$C_T(x, t) = \sum_{n=1}^{\infty} b_n \sin\left(\frac{n\pi x}{L}\right) e^{-t(D(\frac{n\pi}{L})^2 + k)} \quad \text{--- (T3)}$$

Now we can apply $t=0 \rightarrow C_T = -C_0(x)$,

$$\sum_{n=1}^{\infty} b_n \sin\left(\frac{n\pi x}{L}\right) = -C_0 \frac{\sinh\left(\sqrt{\frac{k}{D}}(L-x)\right)}{\sinh\left(\sqrt{\frac{k}{D}}L\right)}$$

↳ fourier sine series!

Using orthogonality

$$b_n = \frac{2}{L} \int_0^L -C_0(x) \sin\left(\frac{n\pi x}{L}\right) dx$$

Using wolfram Alpha for this one

$$b_n = -\frac{2C_0 n\pi}{L^2 \left(\frac{k}{D} + \left(\frac{n\pi}{L}\right)^2\right)} \quad \text{--- (T4)}$$

Finally putting together everything

$$C(x,t) = C_{\infty}(x) + C_+(x,t)$$

$$C(x,t) = C_0 \frac{\sinh\left(\sqrt{\frac{k}{D}}(L-x)\right)}{\sinh\left(\sqrt{\frac{k}{D}}L\right)} - \sum_{n=1}^{\infty} \frac{2 \cos n\pi}{L^2 \left(\frac{k}{D} + \left(\frac{n\pi}{L}\right)^2\right)} \sin\left(\frac{n\pi x}{L}\right) e^{-t \left(D \left(\frac{n\pi}{L}\right)^2 + k\right)}$$

The final solution